theories/SpecNotations.v
@@ -7,4 +7,4 @@ Notation "⊢ v 'in' t" := (Jv v t) (at level 90).
 
 Notation "v0 ⇓ v1" := (big v0 v1) (at level 90).
 
-Notation "Δ ⊢ E [ v ]" := (sat Δ E v) (at level 90).
+Notation "σ |- c 'in' E [ v ]" := (sat σ c E v) (at level 90).
